\chapter[10]

\problem

We consider small perturbation in Minkowski metric
%
\begin{equation}
    g_{\mu\nu} = \eta_{\mu\nu} + h_{\mu\nu}
\end{equation}
%
where $|h_{\mu\nu}| \ll 1$ \\
%
$g^{\mu\nu} = \eta^{\mu\nu} - h^{\mu\nu}$ is indeed inverse of metric
%
\begin{equation}
    \delta\indices{^\mu_\sigma} = g^{\mu\nu}g_{\nu\sigma} =
    (\eta^{\mu\nu} + h^{\mu\nu})(\eta_{\nu\sigma} - h_{\nu\sigma}) =
    \eta^{\mu\nu}\eta_{\nu\sigma} - \eta^{\mu\nu}h_{\nu\sigma} +
    h^{\mu\nu}\eta_{\nu\sigma} - \underbrace{h^{\mu\nu}h_{\nu\sigma}}_{=0}.
\end{equation}
%
We keep only linear terms in $h_{\mu\nu}$. Let's take a look at
%
\begin{equation}
    -\eta^{\mu\nu}h_{\nu\sigma} + h^{\mu\nu}\eta_{\nu\sigma} =
    -\eta^{\mu\nu}h_{\nu\sigma} +
    \eta_{\nu\sigma}\eta^{\nu\beta}\eta^{\mu\alpha}h_{\alpha\beta} =
    -\eta^{\mu\nu}h_{\nu\sigma} +
    \delta\indices{_\sigma^\beta}\eta^{\mu\alpha}h_{\alpha\beta} =
    -\eta^{\mu\nu}h_{\nu\sigma} + \eta^{\mu\alpha}h_{\alpha\sigma} = 0.
\end{equation}
%
So
%
\begin{equation}
    g^{\mu\nu}g_{\nu\sigma} = \eta^{\mu\nu}\eta_{\nu\sigma} = \delta\indices{^\mu_\sigma}.
\end{equation}
%
\problem
%
TT coordinates are defined by following conditions
%
\begin{equation}
    h_{\mu0} = 0 \quad h\indices{^i_i} = 0 \quad \partial_i h^{ij} = 0.
\end{equation}
%
Those coordinates are comoving coordinates to particles initially at rest.
%
\subproblem
%
To prove that I first recall geodesic equation
%
\begin{equation}
    \frac{\dd^2 x^\mu}{\dd \tau^2} +
    \Gamma\indices{^\mu_\alpha_\beta}
    \frac{\dd x^\alpha}{\dd \tau}
    \frac{\dd x^\beta}{\dd \tau} = 0.
\end{equation}
%
Now I expand it in $\tau = 0$ using $\frac{\dd x^i}{\dd \tau} \big|_{\tau=0} =
    0$ :
%
\begin{equation}
    \frac{\dd^2 x^\mu}{\dd \tau^2} \Bigg|_{\tau=0} +
    \Gamma\indices{^\mu_0_0}
    \left(\frac{\dd t}{\dd \tau}\right)^2 \Bigg|_{\tau=0} = 0.
\end{equation}
Now I calculate $\Gamma\indices{^\mu_0_0}$
%
\begin{equation}
    \Gamma\indices{^\mu_0_0} = \frac{1}{2}g^{\mu m}\left(
    \partial_0 g_{m0} +
    \partial_0 g_{m0} -
    \partial_m g_{00}
    \right) =
    \frac{1}{2}g^{\mu m}\left(
    \partial_0 h_{m0} +
    \partial_0 h_{m0} -
    \partial_m h_{00}
    \right) = 0
\end{equation}
%
using $\partial_\mu \eta_{\alpha\beta} = 0$ and $h_{\mu0} = 0$. So now it is
visible that for resting particle there is no change in velocity ($\frac{\dd^2
        x^\mu}{\dd \tau^2} \big|_{\tau=0} = 0$) which means that particle stays in
place.
%
\subproblem
%
Now what is left is to show that proper time is the same as coordinate time. For
this I will calculate
%
\begin{equation}
    \dd \tau = \sqrt{-g_{\mu\nu}\dd x^\mu \dd x^\nu}.
\end{equation}
%
In our case particle is at rest
%
\begin{equation}
    \dd \tau = \sqrt{-g_{00}\dd t^2} =
    \dd t \sqrt{-\eta_{00}-\smash[b]{\underbrace{h_{00}}_{=0}}} =
    \dd t \sqrt{-\eta_{00}} = \dd t
\end{equation}
%
\problem
%
We have given
%
\begin{equation}
    h_{\mu\nu} =
    \begin{pmatrix}
        0 & 0        & 0        & 0 \\
        0 & h_+      & h_\times & 0 \\
        0 & h_\times & -h_+     & 0 \\
        0 & 0        & 0        & 0
    \end{pmatrix}
    \cos\omega(t-z)
\end{equation}
%
\subproblem
%
$\rightarrow$ It is clear that $h_{\mu0} = 0$. \\
$\rightarrow$ To calculate trace I expand
%
\begin{multline}
    h\indices{^i_i} = \eta^{ij}h_{ji} = \Tr
    \left(\begin{pmatrix}
            0 & 0        & 0        & 0 \\
            0 & h_+      & h_\times & 0 \\
            0 & h_\times & -h_+     & 0 \\
            0 & 0        & 0        & 0
        \end{pmatrix}
    \begin{pmatrix}
            -1 & 0 & 0 & 0 \\
            0  & 1 & 0 & 0 \\
            0  & 0 & 1 & 0 \\
            0  & 0 & 0 & 1
        \end{pmatrix}\right)\cos\omega(t-z)=\\
    \cos\omega(t-z)\Tr
    \begin{pmatrix}
        0 & 0        & 0        & 0 \\
        0 & h_+      & h_\times & 0 \\
        0 & h_\times & -h_+     & 0 \\
        0 & 0        & 0        & 0
    \end{pmatrix} = 0
\end{multline}
%
$\rightarrow$ $h_{\mu\nu}$ depends only on $t$ and $z$
\begin{equation}
    \partial_i h^{ij} =
    \eta^{\alpha i}\eta^{\beta j} \partial_i h_{\alpha\beta} =
    \eta^{\alpha t}\eta^{\beta j} \partial_t h_{\alpha\beta} +
    \eta^{\alpha z}\eta^{\beta j} \partial_z h_{\alpha\beta} =
    \eta^{t t}\eta^{\beta j} \partial_t \underbrace{h_{t \beta}}_{=0} +
    \eta^{z z}\eta^{\beta j} \partial_z \underbrace{h_{z \beta}}_{=0} =0
\end{equation}
%
\subproblem
%
\begin{itemize}
    \item $x^\mu_1 = (t,-\frac{L}{2},0,0) \quad x^\mu_2 = (t,\frac{L}{2},0,0)
              \quad \rightarrow \quad
              \Delta x^\mu = (0,L,0,0)$
          %
          \begin{equation}
              \Delta s = \sqrt{g_{\mu\nu}\Delta x^\mu\Delta x^\nu} =
              \sqrt{g_{xx}L^2} =
              L \sqrt{1+h_+\cos\omega(t-z)}
          \end{equation}
          %
    \item $x^\mu_1 = (t,0,-\frac{L}{2},0) \quad x^\mu_2 = (t,0,\frac{L}{2},0)
              \quad \rightarrow \quad
              \Delta x^\mu = (0,L,0,0)$
          %
          \begin{equation}
              \Delta s = \sqrt{g_{\mu\nu}\Delta x^\mu\Delta x^\nu} =
              \sqrt{g_{yy}L^2} =
              L \sqrt{1 - h_+\cos\omega(t-z)}
          \end{equation}
          %
    \item $x^\mu_1 = (t,-\frac{L}{2\sqrt{2}},-\frac{L}{2\sqrt{2}},0) \quad
              x^\mu_2 = (t,\frac{L}{2\sqrt{2}},\frac{L}{2\sqrt{2}},0)
              \quad \rightarrow \quad
              \Delta x^\mu = (0,\frac{L}{\sqrt{2}},\frac{L}{\sqrt{2}},0)$
          %
          \begin{multline}
              \Delta s = \sqrt{g_{\mu\nu}\Delta x^\mu\Delta x^\nu} =
              \sqrt{g_{xx}\frac{L^2}{2} + g_{yy}\frac{L^2}{2} + g_{xy}L^2} = \\
              L\sqrt{(1 + h_+\cos\omega(t-z))\frac{1}{2} +
                  (1 - h_+\cos\omega(t-z))\frac{1}{2} +
                  1 + h_\times \cos\omega(t-z)} = \\
              L\sqrt{2 + h_\times \cos\omega(t-z)}
          \end{multline}
          %
    \item $x^\mu_1 = (t,-\frac{L}{2\sqrt{2}},\frac{L}{2\sqrt{2}},0) \quad
              x^\mu_2 = (t,\frac{L}{2\sqrt{2}},-\frac{L}{2\sqrt{2}},0)
              \quad \rightarrow \quad
              \Delta x^\mu = (0,\frac{L}{\sqrt{2}},-\frac{L}{\sqrt{2}},0)$
          %
          \begin{multline}
              \Delta s = \sqrt{g_{\mu\nu}\Delta x^\mu\Delta x^\nu} =
              \sqrt{g_{xx}\frac{L^2}{2} + g_{yy}\frac{L^2}{2} - g_{xy}L^2} = \\
              L\sqrt{(1 + h_+\cos\omega(t-z))\frac{1}{2} +
                  (1 - h_+\cos\omega(t-z))\frac{1}{2} -
                  1 - h_\times \cos\omega(t-z)} = \\
              L\sqrt{-h_\times \cos\omega(t-z)}
          \end{multline}

\end{itemize}